src/casemate-check-rocq/theories/model.v
@@ -98,11 +98,11 @@ Inductive pte_rec :=
 Record ghost_exploded_descriptor := mk_ghost_exploded_descriptor {
   ged_ia_region : ghost_addr_range;
   ged_level : level_t;
-  ged_stage : stage_t;
+  ged_stage : entry_stage_t;
   ged_pte_kind : pte_rec;
   ged_state : sm_pte_state;
   (* address of the root of the PTE *)
-  ged_owner : owner_t;
+  ged_owner : sm_owner_t;
 }.
 #[export] Instance eta_ghost_exploded_descriptor : Settable _ :=
   settable! mk_ghost_exploded_descriptor <ged_ia_region; ged_level; ged_stage; ged_pte_kind; ged_state; ged_owner>.
@@ -120,49 +120,67 @@ Record sm_location := mk_sm_location {
 
 Record owner_locks := {
   ol_len : u64;
-  ol_owner_ids : list owner_t;
+  ol_owner_ids : list sm_owner_t;
   ol_locks : unit;
 }.
 
+Record cm_root := {
+  r_baddr : sm_owner_t;
+  r_id : addr_id_t;
+  r_refcount : u64;
+}.
+
+Record thrd_ctxt := {
+  current_s1 : sm_owner_t;
+  current_s2 : sm_owner_t;
+}.
+
 (* The memory state is a map from address to simplified model location *)
-Definition casemate_model_state := cmap sm_location.
+Definition casemate_model_memory := cmap sm_location.
 
 (* The memory initialised is stored here *)
 Definition casemate_model_initialised := zmap unit.
 
-(* the map from root to lock address *)
-Definition casemate_model_lock_addr := zmap u64.
+(* per-CPU thread-local context *)
+Definition casemate_model_thrd_ctxt := list thrd_ctxt.
 
-(* the map from lock address to thread that acquired it if any *)
-Definition casemate_model_lock_state := zmap thread_identifier.
+(* Map of pgtable root to lock that owns it *)
+Definition casemate_model_lock_owner_map := zmap u64.
+
+(* Map from the locks to the thread_identifier that has acquired it *)
+Definition casemate_model_lock_state_map := zmap thread_identifier.
 
 Inductive write_authorization :=
   | write_authorized
   | write_unauthorized
 .
 
+(* Map of the locks to the write authorization state *)
 Definition casemate_model_lock_write_authorization := zmap write_authorization.
 
 (* Storing roots for PTE walkthrough (we might need to distinguish S1 and S2 roots) *)
+
+(* TODO: sm_owner_t to cm_root *)
 Record pte_roots := mk_pte_roots {
-  pr_s1 : list owner_t;
-  pr_s2 : list owner_t;
+  pr_s1 : list sm_owner_t;
+  pr_s2 : list sm_owner_t;
 }.
 #[export] Instance eta_pte_roots : Settable _ := settable! mk_pte_roots <pr_s1; pr_s2>.
 
-Record casemate_model := mk_casemate_model {
+Record casemate_model_state := mk_casemate_model_state {
   cm_roots : pte_roots;
-  cm_memory : casemate_model_state;
+  cm_memory : casemate_model_memory;
   cm_initialised : casemate_model_initialised;
-  cm_lock_addr : casemate_model_lock_addr;
-  cm_lock_state : casemate_model_lock_state;
+  cm_thrd_ctxt : casemate_model_thrd_ctxt;
+  cm_lock_addr : casemate_model_lock_owner_map;
+  cm_lock_state : casemate_model_lock_state_map;
   cm_lock_authorization : casemate_model_lock_write_authorization
 }.
-#[export] Instance eta_casemate_model : Settable _ :=
-  settable! mk_casemate_model
-    <cm_roots; cm_memory; cm_initialised; cm_lock_addr; cm_lock_state; cm_lock_authorization>.
+#[export] Instance eta_casemate_model_state : Settable _ :=
+  settable! mk_casemate_model_state
+    <cm_roots; cm_memory; cm_initialised; cm_thrd_ctxt; cm_lock_addr; cm_lock_state; cm_lock_authorization>.
 
-Definition is_initialised (st : casemate_model) (addr : phys_addr_t) : bool :=
+Definition is_initialised (st : casemate_model_state) (addr : phys_addr_t) : bool :=
   match st.(cm_initialised) !! ((bv_shiftr_64 (phys_addr_val addr) b12)) with
     | Some _ => true
     | None => false
@@ -170,7 +188,7 @@ Definition is_initialised (st : casemate_model) (addr : phys_addr_t) : bool :=
 .
 
 Definition get_location
-  (st : casemate_model)
+  (st : casemate_model_state)
   (addr : phys_addr_t) : option sm_location :=
   match st.(cm_memory) !! bv_shiftr_64 (phys_addr_val addr) b3 with
   | Some loc => Some loc
@@ -183,8 +201,8 @@ Definition get_location
 .
 
 Definition get_lock_of_owner
-  (owner : owner_t)
-  (cm : casemate_model) : option u64 :=
+  (owner : sm_owner_t)
+  (cm : casemate_model_state) : option u64 :=
   lookup (phys_addr_val (root_val owner)) cm.(cm_lock_addr).
 
 
@@ -193,7 +211,7 @@ Infix "!!" := get_location (at level 20).
 Definition is_loc_thread_owned
   (cpu : thread_identifier)
   (location : sm_location)
-  (cm : casemate_model) : bool :=
+  (cm : casemate_model_state) : bool :=
   match location.(sl_pte), location.(sl_thread_owner) with
   | Some _, Some thread_owner =>
     bool_decide (thread_owner = cpu)
@@ -204,7 +222,7 @@ Definition is_loc_thread_owned
 Definition is_pte_well_locked
   (cpu : thread_identifier)
   (pte : ghost_exploded_descriptor)
-  (cm : casemate_model) : bool :=
+  (cm : casemate_model_state) : bool :=
   match get_lock_of_owner pte.(ged_owner) cm with
   | None => false
   | Some addr =>
@@ -218,7 +236,7 @@ Definition is_pte_well_locked
 Definition should_visit
   (cpu : thread_identifier)
   (addr : phys_addr_t)
-  (cm : casemate_model) : bool :=
+  (cm : casemate_model_state) : bool :=
   match cm !! addr with
   | None => true
   | Some location =>
@@ -257,18 +275,18 @@ Inductive casemate_model_error :=
 
 Record casemate_model_result := mk_casemate_model_result {
   cmr_log : list log_element;
-  cmr_data : result casemate_model casemate_model_error
+  cmr_data : result casemate_model_state casemate_model_error
 }.
 
 #[export] Instance eta_casemate_model_result : Settable _ :=
   settable! mk_casemate_model_result <cmr_log; cmr_data>.
 
-Definition Mreturn (cm : casemate_model) : casemate_model_result :=
+Definition Mreturn (cm : casemate_model_state) : casemate_model_result :=
   {| cmr_log := nil; cmr_data := Ok _ _ cm |}.
 
 Definition Mbind
   (r : casemate_model_result)
-  (f : casemate_model -> casemate_model_result) :
+  (f : casemate_model_state -> casemate_model_result) :
   casemate_model_result :=
   match r.(cmr_data) with
   | Error _ _ e => r
@@ -287,7 +305,7 @@ Definition Mlog
   r <|cmr_log := s :: r.(cmr_log) |>.
 
 Definition Mupdate_state
-  (updater : casemate_model -> casemate_model_result)
+  (updater : casemate_model_state -> casemate_model_result)
   (st : casemate_model_result) :
   casemate_model_result :=
   match st with
@@ -300,7 +318,7 @@ Definition Mupdate_state
 
 Definition insert_location
   (loc : sm_location)
-  (cm : casemate_model) : casemate_model :=
+  (cm : casemate_model_state) : casemate_model_state :=
   (cm <| cm_memory := <[ loc.(sl_phys_addr) := loc ]> cm.(cm_memory) |>)
 .
 
@@ -317,20 +335,4 @@ Definition Minsert_location
   | e => e
   end
 .
-
-(** States about page tables *)
-
-(* Type used as input of the page table visitor function  *)
-Record page_table_context := mk_page_table_context {
-  ptc_state: casemate_model;
-  ptc_loc: option sm_location;
-  ptc_partial_ia: phys_addr_t;
-  ptc_addr: phys_addr_t;
-  ptc_root: owner_t;
-  ptc_level: level_t;
-  ptc_stage: stage_t;
-}.
-#[export] Instance eta_page_table_context : Settable _ :=
-  settable! mk_page_table_context <ptc_state; ptc_loc; ptc_partial_ia; ptc_addr; ptc_root; ptc_level; ptc_stage>.
-
 
